Test.thy
@@ -6,6 +6,9 @@ begin
 abbreviation p0 :: exp where "p0 \<equiv> Binary Add (Const (ScalarC (IntC 1))) (Const (ScalarC (IntC 2)))"
 abbreviation p1 :: exp where "p1 \<equiv> Unary Inc (Const (ScalarC (IntC 2)))"
 abbreviation p2 :: exp where "p2 \<equiv> Array [p0, p1]"
+abbreviation p3 :: exp where "p3 \<equiv> Array [(Const (ScalarC (IntC 1))), (Const (ScalarC (IntC 2))),
+                                          (Const (ScalarC (IntC 3))), (Const (ScalarC (IntC 4))),
+                                          (Const (ScalarC (IntC 5))), (Const (ScalarC (IntC 6)))]"
 theorem "eval (Map x (Unary Inc (Var x)) p2) = 
          Res (ArrayC [(ScalarC (IntC 4)), (ScalarC (IntC 4))])"
 by fastforce
@@ -28,3 +31,22 @@ theorem "eval (Split (Const (ScalarC (IntC 2)))
                       Const (ScalarC (IntC 3)), Const (ScalarC (IntC 4))])) =
          Res (ArrayC [ArrayC [ScalarC (IntC 1), ScalarC (IntC 2)], ArrayC [ScalarC (IntC 3), ScalarC (IntC 4)]])"
 by normalization
+
+value "eval (Split (Const (ScalarC (IntC 2))) p3)"
+value "eval (Join (Split (Const (ScalarC (IntC 2))) p3))"
+value "eval p3"
+theorem "eval p3 = eval (Join (Split (Const (ScalarC (IntC 2))) p3))"
+by normalization
+
+value "eval (Split (Const (ScalarC (IntC 1))) p3)"
+
+theorem splitjoin: 
+assumes 1: "n > 0"
+assumes 2: "e = (Const (ArrayC a))"
+assumes 3: "e' = (Join (Split (Const (ScalarC (IntC n))) (Const (ArrayC a))))"
+shows "eval e' = eval e"
+using 1 2 3
+apply auto
+sorry
+
+end
